Chapter 7: Exercise 1
=====================

## a
For $x \le \xi$, $f_1(x)$ has coefficients
$a_1 = \beta_0, b_1 = \beta_1, c_1 = \beta_2, d_1 = \beta_3$.

## b
For $x \gt \xi$, $f(x)$ has the form of:
$$
\beta_0 + \beta_1 x + \beta_2 x^2 + \beta_3 x^3 + \beta_4 (x - \xi)^3
\\
= \beta_0 + \beta_1 x + \beta_2 x^2 + \beta_3 x^3 + \beta_4 (x^3 - 3 x^2 \xi + 3 x \xi^2 - \xi^3)
\\
= (\beta_0 - \beta_4 \xi^3) + (\beta_1 + 3 \beta_4 \xi^2) x + (\beta_2 - 3 \beta_4 \xi) x^2 + (\beta_3 + \beta_4) x^3
$$

Thus, $a_2 = \beta_0 - \beta_4 \xi^3, b_2 = \beta_1 + 3 \beta_4 \xi^2, c_2 = \beta_2 - 3 \beta_4 \xi, d_2 = \beta_3 + \beta_4$.

## c
$$
f_1(\xi) = \beta_0 + \beta_1 \xi + \beta_2 \xi^2 + \beta_3 \xi^3
\\
f_2(\xi) = (\beta_0 - \beta_4 \xi^3) + (\beta_1 + 3 \beta_4 \xi^2) \xi + (\beta_2 - 3 \beta_4 \xi) \xi^2 + (\beta_3 + \beta_4) \xi^3
\\
= \beta_0 - \beta_4 \xi^3 + \beta_1 \xi + 3 \beta_4 \xi^3 + \beta_2 \xi^2 - 3 \beta_4 \xi^3 + \beta_3 \xi^3 + \beta_4 \xi^3
\\
= \beta_0 + \beta_1 \xi + \beta_2 \xi^2 + 3 \beta_4 \xi^3 - 3 \beta_4 \xi^3 + \beta_3 \xi^3 + \beta_4 \xi^3 - \beta_4 \xi^3
\\
= \beta_0 + \beta_1 \xi + \beta_2 \xi^2 + \beta_3 \xi^3
$$

## d 
$$
f'(x) = b_1 + 2 c_1 x + 3 d_1 x^2 
\\
f_1'(\xi) = \beta_1 + 2 \beta_2 \xi + 3 \beta_3 \xi^2
\\
f_2'(\xi) = \beta_1 + 3 \beta_4 \xi^2 + 2 (\beta_2 - 3 \beta_4 \xi) \xi + 3 (\beta_3 + \beta_4) \xi^2
\\
= \beta_1 + 3 \beta_4 \xi^2 + 2 \beta_2 \xi - 6 \beta_4 \xi^2 + 3 \beta_3 \xi^2 + 3 \beta_4 \xi^2
\\
= \beta_1 + 2 \beta_2 \xi + 3 \beta_3 \xi^2 + 3 \beta_4 \xi^2 + 3 \beta_4 \xi^2 - 6 \beta_4 \xi^2 
\\
= \beta_1 + 2 \beta_2 \xi + 3 \beta_3 \xi^2
$$


## e
$$
f''(x) = 2 c_1 + 6 d_1 x
\\
f_1''(\xi) = 2 \beta_2 + 6 \beta_3 \xi
\\
f_2''(\xi) = 2 (\beta_2 - 3 \beta_4 \xi) + 6 (\beta_3 + \beta_4) \xi
\\
= 2 \beta_2 + 6 \beta_3 \xi
$$
