---
title: "Chapter 10: Exercise 1"
output: html_document
---

### a
Proof of Equation (10.12) $$
\frac{1}{|C_k|} \sum\limits_{i,i^{\prime} \in C_k} \sum\limits_{j=1}^p (x_{ij} - x_{i^\prime j})^2 = 
2 \sum\limits_{i \in C_k} \sum\limits_{j=1}^{p} (x_{ij} - \bar{x}_{kj})^2
\\
= \frac{1}{|C_k|} \sum\limits_{i,i^{\prime} \in C_k} \sum\limits_{j=1}^p ((x_{ij} - \bar{x}_{kj}) - (x_{i^\prime j} - \bar{x}_{kj}))^2
\\
= \frac{1}{|C_k|} \sum\limits_{i,i^{\prime} \in C_k} \sum\limits_{j=1}^p ((x_{ij} - \bar{x}_{kj})^2 - 2 (x_{ij} - \bar{x}_{kj})(x_{i^\prime j} - \bar{x}_{kj}) + (x_{i^\prime j} - \bar{x}_{kj})^2)
\\
= \frac{|C_k|}{|C_k|} \sum\limits_{i \in C_k} \sum\limits_{j=1}^p (x_{ij} - \bar{x}_{kj})^2 +
  \frac{|C_k|}{|C_k|} \sum\limits_{i^{\prime} \in C_k} \sum\limits_{j=1}^p (x_{i^\prime j} - \bar{x}_{kj})^2 -
  \frac{2}{|C_k|} \sum\limits_{i,i^{\prime} \in C_k} \sum\limits_{j=1}^p (x_{ij} - \bar{x}_{kj})(x_{i^\prime j} - \bar{x}_{kj})
\\
= 2 \sum\limits_{i \in C_k} \sum\limits_{j=1}^p (x_{ij} - \bar{x}_{kj})^2 + 0
$$

### b
Equation (10.12) shows that minimizing the sum of the squared Euclidean
distance for each cluster is the same as minimizing the within-cluster variance
for each cluster.