1
========================================================

$$
(4.2) p(X) = \frac {e^{\beta_0 + \beta_1 X}} {1 + e^{\beta_0 + \beta_1 X}}
$$

So, $\frac {p(X)} {1 - p(X)}$

$$
= \frac {\frac {e^{\beta_0 + \beta_1 X}} {1 + e^{\beta_0 + \beta_1 X}}}
        {1 - \frac {e^{\beta_0 + \beta_1 X}} {1 + e^{\beta_0 + \beta_1 X}}}
\\
= \frac {\frac {e^{\beta_0 + \beta_1 X}} {1 + e^{\beta_0 + \beta_1 X}}}
        {
          \frac {1 + e^{\beta_0 + \beta_1 X}} {1 + e^{\beta_0 + \beta_1 X}}
          - \frac {e^{\beta_0 + \beta_1 X}} {1 + e^{\beta_0 + \beta_1 X}}
        }
\\
= \frac {\frac {e^{\beta_0 + \beta_1 X}} {1 + e^{\beta_0 + \beta_1 X}}}
        {\frac {1} {1 + e^{\beta_0 + \beta_1 X}}}
\\
(4.3)    \frac {p(X)} {1 - p(X)} =e^{\beta_0 + \beta_1 X}
$$
