3
========================================================

$$
p_k(x) = \frac {\pi_k
                \frac {1} {\sqrt{2 \pi} \sigma_k}
                \exp(- \frac {1} {2 \sigma_k^2} (x - \mu_k)^2)
               }
               {\sum {
                \pi_l
                \frac {1} {\sqrt{2 \pi} \sigma_l}
                \exp(- \frac {1} {2 \sigma_l^2} (x - \mu_l)^2)
               }}
\\
\log(p_k(x)) = \frac {\log(\pi_k) +
                \log(\frac {1} {\sqrt{2 \pi} \sigma_k}) + 
                - \frac {1} {2 \sigma_k^2} (x - \mu_k)^2
               }
               {\log(\sum {
                \pi_l
                \frac {1} {\sqrt{2 \pi} \sigma_l}
                \exp(- \frac {1} {2 \sigma_l^2} (x - \mu_l)^2)
               })}
\\
\log(p_k(x)) 
\log(\sum {
     \pi_l
     \frac {1} {\sqrt{2 \pi} \sigma_l}
     \exp(- \frac {1} {2 \sigma_l^2} (x - \mu_l)^2)
    })
= \log(\pi_k) +
  \log(\frac {1} {\sqrt{2 \pi} \sigma_k}) + 
  - \frac {1} {2 \sigma_k^2} (x - \mu_k)^2    
\\
\delta(x)
= \log(\pi_k) +
  \log(\frac {1} {\sqrt{2 \pi} \sigma_k}) + 
  - \frac {1} {2 \sigma_k^2} (x - \mu_k)^2 
$$

As you can see, $\delta(x)$ is a quadratic function of $x$.

